Classes/Galois.v
@@ -3,7 +3,7 @@ Require Import Classes.Joinable.
 Require Import Instances.Preorder.
 Require Import PreorderedSet.
 
-Class Galois (A A' : Type) `{PreorderedSet A'} : Type :=
+Class Galois (A A' : Type) `{A'_preorder: PreorderedSet A'} : Type :=
 {
   gamma : A' -> A -> Prop;
   gamma_monotone : monotone gamma;
@@ -16,8 +16,8 @@ Ltac gamma_destruct := repeat
   | x : gamma _  _ |- _ => inv x
   end.
 
-Lemma gamma_preorder {A B} `{Galois B A}: forall (a a' : A) (b : B), 
-    preorder a a' -> gamma a b -> gamma a' b.
+Lemma gamma_preorder {A A'} `{A_galois : Galois A A'}: forall (a' a2' : A') (a : A), 
+    preorder a' a2' -> gamma a' a -> gamma a2' a.
 Proof.
   intros a a' b Hpre Hgamma.
   pose proof gamma_monotone as Hmono.
@@ -25,18 +25,20 @@ Proof.
   destruct Hpre. auto with soundness.
 Qed.
 
-Lemma gamma_join_left {A A'} `{Joinable A'} `{_ : @Galois A A' H} : ∀ (a : A) (a'1 a'2 : A'),
+Lemma gamma_join_left {A A'} `{A'_joinable : Joinable A'} 
+  `{A_galois : @Galois A A' T_preorder} : ∀ (a : A) (a'1 a'2 : A'),
   gamma a'1 a → gamma (join_op a'1 a'2) a.
 Proof. 
   intros. apply (gamma_preorder a'1). 
   apply join_upper_bound_left. assumption.
 Qed.
 
-Lemma gamma_join_right {A A'} `{Joinable A'} `{_ : @Galois A A' H} : ∀ (a : A) (a'1 a'2 : A'),
+Lemma gamma_join_right {A A'} `{A'_joinable : Joinable A'} 
+  `{A_galois : @Galois A A' T_preorder} : ∀ (a : A) (a'1 a'2 : A'),
   gamma a'2 a → gamma (join_op a'1 a'2) a.
 Proof. 
-  intros. apply (gamma_preorder a'2). apply join_upper_bound_right.
-  assumption.
+  intros. apply (gamma_preorder a'2). 
+  apply join_upper_bound_right. assumption.
 Qed.
 
 Ltac apply_widen :=
