Classes/Monad/MonadFail.v
@@ -3,12 +3,12 @@ Require Import Classes.Monad.
 Require Import Classes.Applicative.
 Require Import Classes.Galois.
 
-Class MonadFail M `{Monad M} : Type := {
+Class MonadFail M `{M_monad : Monad M} : Type := {
   fail {A : Type} : M A;
   fail_left: ∀ {A B} (m : A → M B), (@fail A) >>= m = fail;
 }.
 Arguments fail : simpl never.
 Hint Rewrite @fail_left : soundness.
 
-Definition guard {M} `{MonadFail M} : bool → M unit := 
+Definition guard {M} `{M_fail : MonadFail M} : bool → M unit := 
   λ b, if b then skip else fail.
