Classes/SoundMonad.v
@@ -8,18 +8,18 @@ Require Import Classes.Monad.MonadFail.
 Require Import Instances.Galois.
 
 Section sound_monad.
-  Context (M M' : Type → Type) `{MonadFail M, MonadFail M'}.
+  Context (M M' : Type → Type) `{M_fail : MonadFail M, M'_fail : MonadFail M'}.
   Context {M_preorder : ∀ T', PreorderedSet T' → PreorderedSet (M' T')}.
   Context {M_galois : ∀ T T' {HT : PreorderedSet T'}, Galois T T' → Galois (M T) (M' T')}.
 
   Class SoundMonad : Type :=
   {
     fmap_sound : ∀ (A A' B B' : Type) `{Galois A A', Galois B B'},
-      gamma (fmap (F:=M') (A:=A') (B:=B')) (fmap (F:=M) (A:=A) (B:=B));
+      gamma (fmap (M:=M') (A:=A') (B:=B')) (fmap (M:=M) (A:=A) (B:=B));
     pure_sound : ∀ (A A' : Type) `{Galois A A'},
-      gamma (pure (F:=M') (A:=A')) (pure (F:=M) (A:=A));
+      gamma (pure (M:=M') (A:=A')) (pure (M:=M) (A:=A));
     app_sound : ∀ (A A' B B' : Type) `{Galois A A', Galois B B'},
-      gamma (app (F:=M') (A:=A') (B:=B')) (app (F:=M) (A:=A) (B:=B));
+      gamma (app (M:=M') (A:=A') (B:=B')) (app (M:=M) (A:=A) (B:=B));
     bind_sound : ∀ (A A' B B' : Type) `{Galois A A', Galois B B'},
       gamma (bindM (M:=M') (A:=A') (B:=B')) (bindM (M:=M) (A:=A) (B:=B));
     gamma_fail : ∀ (A A' : Type) `{Galois A A'} (m : M A), gamma fail m;
