Instances/IsBool/Boolean.v
@@ -8,28 +8,28 @@ Require Import Classes.Applicative.
 
 Generalizable Variable M.
 
-Definition ensure_bool `{MonadFail M} (v : cvalue) : M bool :=
+Definition ensure_bool `{M_monad : MonadFail M} (v : cvalue) : M bool :=
   match v with
   | VBool b => pure b
   | _ => fail
   end.
 
-Definition build_boolean `{Monad M} (b : bool) : M cvalue :=
+Definition build_boolean `{M_monad : Monad M} (b : bool) : M cvalue :=
   pure (VBool b).
 
-Definition extract_boolean `{Monad M} (b : bool) : M bool :=
+Definition extract_boolean `{M_monad : Monad M} (b : bool) : M bool :=
   pure b.
 
-Definition andbM `{Monad M} (b c : bool) : M bool := 
+Definition andbM `{M_monad : Monad M} (b c : bool) : M bool := 
   pure (andb b c).
 
-Definition negbM `{Monad M} (b : bool) : M bool := 
+Definition negbM `{M_monad : Monad M} (b : bool) : M bool := 
   pure (negb b).
 
-Definition eval_if {A} `{Monad M} (b : bool) (st1 st2 : M A) : M A :=
+Definition eval_if {A} `{M_monad : Monad M} (b : bool) (st1 st2 : M A) : M A :=
   if b then st1 else st2.
 
-Instance boolean_type `{MonadFail M} : IsBool M cvalue bool :=
+Instance boolean_type `{M_fail : MonadFail M} : IsBool M cvalue bool :=
 {
   ensure_bool := ensure_bool;
   build_bool := build_boolean;
